\documentclass{article}
\usepackage[english]{babel}
\usepackage[utf8]{inputenc}
\usepackage{amsmath}
\usepackage{amssymb}
\usepackage{amsthm}

\begin{document}

\section{Equality of Sets}
Theorems:

\begin{proof}

$L_1 \times (L_2 \cup L_3) \equiv (L_1 \times L_2) \cup (L_1 \times L_3)$
\\
\\
The proof will be divided into two parts. the first will show that: \newline
$L_1 \times (L_2 \cup L_3) \subseteq (L_1 \times L_2) \cup (L_1 \times L_3)$ \newline
\\
\\
And the second that: \newline
$(L_1 \times L_2) \cup (L_1 \times L_3) \subseteq L_1 \times (L_2 \cup L_3)$ \newline
\\
\\
Proof: \newline
let $w \in L_1 \times (L_2 \cup L_3)$ \newline
\\
  Concatenation definition: \newline 
  $\Longrightarrow \exists y,z \in \Sigma^{*} \mid w = yz ~and~ (y \in L_1) \wedge (z \in (L_2 \cup L_3))$ \newline
  Union definition: \newline 
  $\Longrightarrow \exists y,z \in \Sigma^{*} \mid w = yz ~and~ (y \in L_1) \wedge (z \in L_2 \vee z \in L_3)$ \newline
  Distribution definition: \newline
  $\Longrightarrow \exists y,z \in \Sigma^{*} \mid w = yz ~and ~ (y \in L_1 \wedge z \in L_2) \vee (y \in L_1 \wedge z \in L_3)$ \newline
  Concatenation definition: \newline
  $\Longrightarrow w \in L_1 \times L_2 \vee w \in L_1 \times L_3$ \newline
  Union definition: \newline
  $\Longrightarrow w \in (L_1 \times L_2) \cup (L_1 \times L_3))$ \newline
  Subset definition: \newline 
  $\Longrightarrow L_1 \times (L_2 \cup L_3) \subseteq (L_1 \times L_2) \cup (L_1 \times L_3)$
  \\
  \\
  Let $w \in (L_1 \times L_2) \cup (L_1 \times L_3)$ \newline
\\
Union definition: \newline
  $\Longrightarrow w \in (L_1 \times L_2) \vee w \in (L_1 \times L_3)$ \newline
Concatenation definition: \newline
  $\Longrightarrow \exists y,z \in \Sigma^{*} \mid w = yz ~and~ (y \in L_1 \wedge z \in L_2) \vee (y \in L_1 \wedge z \in L_3)$ \newline
Union definition: \newline
  $\Longrightarrow \exists y,z \in \Sigma^{*} \mid w = yz ~and~ (y \in L_1 \wedge z \in (L_2 \cup L_3))$ \newline
Concatenation definition: \newline
  $\Longrightarrow w \in L_1 \times (L_2 \cup L_3)$ \newline
Subset definition: \newline
  $\Longrightarrow (L_1 \times L_2) \cup (L_1 \times L_3) \subseteq (L_1 \times (L_2 \cup L_3))$ \newline
Group equality definition: \newline
$\Longrightarrow L_1 \times (L_2 \cup L_3) \equiv (L_1 \times L_2) \cup (L_1 \times L_3)$ \newline

\end{proof}
\begin{proof}
  $L_1^{*} \cup L_2^{*}(L_1 \cap L_2)^{*} \subseteq (L_1 \cup L_2)^{*}$ \newline
\\
  $~let~ w \in L_1^{*} \cup L_2^{*}(L_1 \cap L_2)^{*}$ \newline
  $~let~ t \in (L_1 \cup L_2)^{*}$ \newline
\\
  Definition of union: \newline
  $\Longrightarrow w \in L_1^{*} \vee w \in L_2^{*}(L_1 \cap L_2)^{*}$


  Differenciating possible circumstances: \newline
  Assume: $w \in L_1^{*}$ \newline
\\
It would be sufficient for such circumstances to prove that: \newline
  $w \in (L_1 \cup L_2)^{*}$ \newline
\\
Proof: \newline
  $w \in L_1^{*}$ \newline
  Definition of Kleene Star: \newline
  $\Longrightarrow w = w_1 \circ w_2 \circ \ldots \circ w_n \mid w_{1,2, \ldots, n} \in L_1$ \newline
  Definition of Union: \newline
  $\Longrightarrow w_{1,2, \ldots, n} \in L_1 \cup L_2$ \newline
  Definition of Kleene Star: \newline
  $\Longrightarrow w_1 \circ w_2 \circ \ldots \circ w_n \in (L_1 \cup L_2)^{*} $ \newline
  Definition of w: \newline
  $\Longrightarrow w \in (L_1 \cup L_2)^{*} $ \newline
\\
  Assume: $w \in L_2^{*}(L_1 \cap L_2)^{*}$ \newline
  \\
  It would be sufficient for such circumstances to prove that: \newline
  $w \in (L_1 \cup L_2)^{*}$ \newline
  Definition of Concatenation: \newline
  $\Longrightarrow \exists y \in L_2^{*} \exists z \in (L_1 \cap L_2)^{*} \mid w = yz$ \newline
  Definition of Kleene Star: \newline
  $\Longrightarrow z = z_1 \circ z_2 \circ \ldots \circ z_n \mid z_{1,2, \ldots, n} \in (L_1 \cap L_2)$ \newline
  Definition of Intersection: \newline
  $\Longrightarrow z_{1,2, \ldots, n} \in L_2$ \newline
  Definition of Kleene Star: \newline
  $\Longrightarrow z \in L_2^{*}$ \newline
  Definition of z: \newline
  $\Longrightarrow \exists y \in L_2^{*} \exists z \in L_2^{*} \mid w = yz$ \newline
  $\Longrightarrow \exists y,z \in L_2^{*} \mid w = yz$ \newline
  Definition of Kleene Star: \newline
  $\Longrightarrow w \in L_2^{*}$ \newline
  Definition of Kleene Star: \newline
  $\Longrightarrow w = w_1 \circ w_2 \circ \ldots \circ w_n | w_{1,2, \ldots, n} \in L_2$ \newline
  Definition of Union: \newline
  $w_{1,2, \ldots, n} \in L_1 \cup L_2 $ \newline
  Definition of Kleene Star: \newline
  $\Longrightarrow w_1 \circ w_2 \circ \ldots \circ w_n \in (L_1 \cup L_2)^{*} $ \newline
  Definition of w: \newline
  $\Longrightarrow w \in (L_1 \cup L_2)^{*} $ \newline

  Proven for all possible circumstances.
  



\end{proof}
\end{document}
